State tree uniqueness separately from upper bound on tags

theories/tree_borrows/defs.v
@@ -13,31 +13,28 @@ Definition wf_mem_tag (h: mem) (nxtp: tag) :=
   ∀ (l l':loc) pid, h !! l = Some (ScPtr l' pid) →
     (pid < nxtp)%nat.
 
-Definition item_wf (it:item) (nxtp:tag) (nxtc:call_id) :=
+Definition wf_item_fresh (it:item) (nxtp:tag) (nxtc:call_id) :=
   (forall tg, IsTag tg it -> (tg < nxtp)%nat)
   /\ (forall cid, protector_is_for_call cid (iprot it) -> (cid < nxtc)%nat).
 
-Definition tree_item_included (tr:tree item) (nxtp:tag) (nxtc: call_id) :=
-  forall tg,
-  tree_contains tg tr -> exists it,
-    tree_unique tg tr
-    /\ tree_item_determined tg it tr
-    /\ item_wf it nxtp nxtc.
-  (* FIXME: unique *)
+Definition wf_tree_fresh (tr:tree item) (nxtp:tag) (nxtc:call_id) :=
+  every_node (fun it => wf_item_fresh it nxtp nxtc) tr.
 
-(* FIXME: consistent naming *)
-Definition wf_tree (tr:tree item) (nxtp:tag) (nxtc:call_id) :=
-  tree_item_included tr nxtp nxtc.
-Definition wf_trees (trs:trees) (nxtp:tag) (nxtc: call_id) :=
-  ∀ blk tr, trs !! blk = Some tr → wf_tree tr nxtp nxtc.
+Definition wf_trees_fresh (trs:trees) (nxtp:tag) (nxtc:call_id) :=
+  ∀ blk tr, trs !! blk = Some tr → wf_tree_fresh tr nxtp nxtc.
+
+Definition wf_tree_nodup (tr:tree item) :=
+  forall tg, tree_contains tg tr -> tree_unique tg tr.
+
+Definition wf_trees_nodup (trs:trees) :=
+  ∀ blk tr, trs !! blk = Some tr → wf_tree_nodup tr.
+
 Definition wf_non_empty (trs:trees) :=
   ∀ blk tr, trs !! blk = Some tr → tr ≠ empty.
-(*
-Definition wf_no_dup (α: stacks) :=
-  ∀ l stk, α !! l = Some stk → NoDup stk.
-*)
+
 Definition wf_cid_incl (cids: call_id_set) (nxtc: call_id) :=
   ∀ c : call_id, c ∈ cids → (c < nxtc)%nat.
+
 Definition wf_scalar t sc := ∀ t' l, sc = ScPtr l t' → t' < t.
 
 (* mem ~ gmap loc scalar
@@ -54,7 +51,8 @@ Record state_wf (s: state) := {
   (*state_wf_dom : dom s.(shp) ≡ dom s.(strs); Do we care ? After all TB is very permissive about the range, so out-of-bounds UB is *always* triggered at the level of the heap, not the trees *)
   state_wf_dom : same_blocks s.(shp) s.(strs);
   (*state_wf_mem_tag : wf_mem_tag s.(shp) s.(snp);*) (* FIXME: this seems to state that all pointers are wf, it should be included *)
-  state_wf_tree_item : wf_trees s.(strs) s.(snp) s.(snc);
+  state_wf_tree_fresh : wf_trees_fresh s.(strs) s.(snp) s.(snc);
+  state_wf_tree_nodup : wf_trees_nodup s.(strs);
   state_wf_non_empty : wf_non_empty s.(strs);
   (*state_wf_cid_no_dup : NoDup s.(scs) ;*) (* FIXME: call ids are unique, include this *)
   state_wf_cid_agree: wf_cid_incl s.(scs) s.(snc);
